[x86] Generalize proofs about memory region functions (and their guards).

books/kestrel/x86/regions.lisp
@@ -12,7 +12,6 @@
 
 ;; See also the function SEPARATE, but this machinery is intended to be more amenable to SMT solving.
 
-;(include-book "projects/x86isa/proofs/utilities/general-memory-utils" :dir :system) ; reduce?  and get rid of ttags
 (include-book "kestrel/bv/bvlt-def" :dir :system)
 (include-book "kestrel/bv/bvminus" :dir :system) ; todo: reduce
 ;(include-book "kestrel/bv/sbvlt-def" :dir :system)
@@ -27,37 +26,43 @@
 ;; START-AD.  Note that the region may wrap around the end of the address
 ;; space, so AD may be in the region even if it is less than START-AD.
 ;; We put the len argument before start-ad because len is often a small constant.
+;; In the normal case (non-huge, non-zero length), this can be opened up to a nice BV claim.
 (defund in-regionp (ad len start-ad)
   (declare (xargs :guard (and (unsigned-byte-p 48 ad)
-                              (unsigned-byte-p 48 len) ; can't be 2^48 as the len gets chopped to 48 bits
+                              (natp len) ; note that len >= 2^48 covers the whole region
                               (unsigned-byte-p 48 start-ad))))
-  (bvlt 48 (bvminus 48 ad start-ad) len))
+  (and (natp len) ; len=0 falsifies the bvlt below
+       (if (<= (expt 2 48) len) ; we handle (expt 2 48) here, since the len gets chopped to 48 bits below
+           t ; the region covers the whole address space
+         (bvlt 48 (bvminus 48 ad start-ad) len))))
 
 ;; Nothing is in a region of size 0
-(defthm not-in-regionp-of-0
+(defthm not-in-regionp-of-0s
   (not (in-regionp ad 0 start-ad))
   :hints (("Goal" :in-theory (enable in-regionp bvuminus bvplus ifix ACL2::BVCHOP-OF-SUM-CASES))))
 
 ;; The address at the start of the region is in the region IFF the size is non-zero
 (defthm in-regionp-same
-  (equal (in-regionp ad size ad)
-         (posp (bvchop 48 size)))
+  (equal (in-regionp ad len ad)
+         (posp len))
   :hints (("Goal" :in-theory (enable in-regionp bvuminus bvplus ifix acl2::bvchop-of-sum-cases zp bvlt))))
 
 ;; The address at the end of the region is in the region IFF the size is non-zero
 (defthm in-regionp-same-end
-  (equal (in-regionp (bvplus 48 ad (bvplus 48 -1 size)) size ad)
-         (posp (bvchop 48 size)))
+  (equal (in-regionp (bvplus 48 ad (bvplus 48 -1 len)) len ad)
+         (posp len))
   :hints (("Goal" :in-theory (enable in-regionp bvuminus bvplus ifix acl2::bvchop-of-sum-cases zp bvlt))))
 
 (defthm in-regionp-same-end-alt
-  (equal (in-regionp (bvplus 48 281474976710655 (bvplus 48 ad size)) size ad)
-         (posp (bvchop 48 size)))
+  (equal (in-regionp (bvplus 48 281474976710655 (bvplus 48 ad len)) len ad)
+         (posp len))
   :hints (("Goal" :in-theory (enable in-regionp bvuminus bvplus ifix acl2::bvchop-of-sum-cases zp bvlt))))
 
 ;; note that the region size can't be 2^48
 (defthm not-in-regionp-one-past-end
-  (not (in-regionp (bvplus 48 ad size) size ad))
+  (equal (in-regionp (bvplus 48 ad len) len ad)
+         (and (<= (expt 2 48) len)
+              (natp len)))
   :hints (("Goal" :in-theory (enable in-regionp bvuminus bvplus ifix acl2::bvchop-of-sum-cases zp bvlt))))
 
 ;; if the region size is 2^48-1, being in the region means not being the single address just before the region
@@ -96,12 +101,14 @@
                   (in-regionp ad len start-ad)))
   :hints (("Goal" :in-theory (enable in-regionp))))
 
-(defthm in-regionp-of-+-arg1
+(defthmd in-regionp-of-+-arg1
   (implies (and (integerp x)
                 (integerp y))
            (equal (in-regionp (+ x y) len ad)
                   (in-regionp (bvplus 48 x y) len ad)))
   :hints (("Goal" :in-theory (enable in-regionp bvplus))))
+
+(theory-invariant (incompatible (:rewrite in-regionp-of-+-arg1) (:definition bvplus)))
 
 (defthmd in-regionp-of-+-arg3
   (implies (and (integerp x)
@@ -161,7 +168,7 @@
 (defthm in-regionp-cancel-1-3
   (equal (in-regionp x len (bvplus 48 y (bvplus 48 z x)))
          (in-regionp 0 len (bvplus 48 y z)))
-  :hints (("Goal" :in-theory (enable in-regionp bvminus bvlt ifix bvplus))))
+  :hints (("Goal" :in-theory (enable in-regionp bvuminus bvminus bvlt ifix bvplus))))
 
 ;; removes the negative part of the range
 (defthm in-regionp-when-non-negative-and-negative-range
@@ -214,7 +221,9 @@
 ;; disabled for the proofs below
 (defthmd in-regionp-of-0-arg3
   (equal (in-regionp ad len 0)
-         (bvlt 48 ad len))
+         (and (natp len)
+              (or (<= (expt 2 48) len)
+                  (bvlt 48 ad len))))
   :hints (("Goal" :in-theory (enable in-regionp))))
 
 (defthm in-regionp-subst-constant-arg1
@@ -227,9 +236,10 @@
 
 (defthmd in-regionp-opener
   (implies (and (not (zp len))
-                (unsigned-byte-p 48 len)
+;                (unsigned-byte-p 48 len)
          ;       (unsigned-byte-p 48 ad)
-                (unsigned-byte-p 48 start-ad))
+                (unsigned-byte-p 48 start-ad)
+                )
            (equal (in-regionp ad len start-ad)
                   (or (equal (bvchop 48 ad) start-ad)
                       (in-regionp ad (+ -1 len) (+ 1 start-ad)))))
@@ -237,21 +247,41 @@
 
 ;;;;;;;;;;;;;;;;;;;;;;;;;;;;;;;;;;;;;;;;;;;;;;;;;;;;;;;;;;;;;;;;;;;;;;;;;;;;;;;;
 
-;; Defines what it means for 2 memory regions to be disjoint.
+;; Defines what it means for 2 memory regions to be disjoint (no address in both regions).
+;; Region1 has size len1 and starts at ad1.
+;; Region2 has size len2 and starts at ad2.
+;; Regions may wrap around the end of the address space back to the start.
 ;; We put the len arguments first because they will often be small constants.
+;; In the normal case, this can be opened up to a conjunction of nice, BV claims.
 (defund disjoint-regionsp (len1 ad1 len2 ad2)
-  (declare (xargs :guard (and (unsigned-byte-p 48 len1) ; can't be 2^48 as the len gets chopped to 48 bits
+  (declare (xargs :guard (and (natp len1) ; note that len >= 2^48 covers the whole region
                               (unsigned-byte-p 48 ad1)
-                              (unsigned-byte-p 48 len2) ; can't be 2^48 as the len gets chopped to 48 bits
+                              (natp len2) ; note that len >= 2^48 covers the whole region
                               (unsigned-byte-p 48 ad2))))
-  (if (or (equal 0 len1)
-          (equal 0 len2))
-      t
-    (and (bvle 48 len1 (bvminus 48 ad2 ad1)) ; the start of region2 is not within region 1  ;; todo: rephrase to use bvlt?
-         (bvle 48 len2 (bvminus 48 ad1 ad2)) ; the start of region1 is not within region 2
-         )))
+  (if (or (zp len1)
+          (zp len2))
+      t ; one region is empty
+    (if (or (<= (expt 2 48) len1)
+            (<= (expt 2 48) len2))
+        nil ; one region covers the whole space (and the other is not empty)
+      ;; Normal case (non-huge, non-empty regions):
+      (and (bvle 48 len1 (bvminus 48 ad2 ad1)) ; the start of region2 is not within region 1  ;; todo: rephrase to use bvlt?
+           (bvle 48 len2 (bvminus 48 ad1 ad2)) ; the start of region1 is not within region 2
+           ))))
 
 ;; todo: more sanity check properties
+
+(defthm disjoint-regionsp-when-not-posp
+  (implies (not (posp len1))
+           (disjoint-regionsp len1 ad1 len2 ad2))
+  :hints (("Goal" :in-theory (enable disjoint-regionsp))))
+
+;; (defthm disjoint-regionsp-when-zp
+;;   (implies (and (zp len1)
+;;                 ;(natp len1) ; drop, have the function nfix
+;;                 )
+;;            (disjoint-regionsp len1 ad1 len2 ad2))
+;;   :hints (("Goal" :in-theory (enable disjoint-regionsp zp))))
 
 (defthmd disjoint-regionsp-symmetric
   (equal (disjoint-regionsp len1 ad1 len2 ad2)
@@ -396,6 +426,8 @@
           (not (and (in-regionp ad len1 ad1)
                     (in-regionp ad len2 ad2)))))
 
+(in-theory (disable disjoint-regionsp-spec))
+
 (defthm disjoint-regionsp-spec-necc-better
   (implies (and (in-regionp ad len1 ad1)
                 (in-regionp ad len2 ad2))
@@ -410,11 +442,53 @@
   :hints (("Goal" :use disjoint-regionsp-spec-necc
            :in-theory (theory 'minimal-theory))))
 
+(encapsulate ()
+  (local (defthmd disjoint-regionsp-spec-of-bvchop-arg2-fw
+           (implies (disjoint-regionsp-spec len1 (bvchop 48 ad1) len2 ad2)
+                    (disjoint-regionsp-spec len1 ad1 len2 ad2))
+           :hints (("Goal" :expand (disjoint-regionsp-spec len1 ad1 len2 ad2)
+                    :in-theory (enable ;disjoint-regionsp-spec
+                                 )))))
+
+  (local (defthmd disjoint-regionsp-spec-of-bvchop-arg2-bk
+           (implies (disjoint-regionsp-spec len1 ad1 len2 ad2)
+                    (disjoint-regionsp-spec len1 (bvchop 48 ad1) len2 ad2))
+           :hints (("Goal"  :expand (disjoint-regionsp-spec len1 (bvchop 48 ad1) len2 ad2)
+                    :in-theory (enable ;disjoint-regionsp-spec
+                                 )))))
+
+  (defthm disjoint-regionsp-spec-of-bvchop-arg2
+    (equal (disjoint-regionsp-spec len1 (bvchop 48 ad1) len2 ad2)
+           (disjoint-regionsp-spec len1 ad1 len2 ad2))
+    :hints (("Goal" :use (disjoint-regionsp-spec-of-bvchop-arg2-fw
+                           disjoint-regionsp-spec-of-bvchop-arg2-bk)))))
+
+(encapsulate ()
+  (local (defthmd disjoint-regionsp-spec-of-bvchop-arg4-fw
+           (implies (disjoint-regionsp-spec len1 ad1 len2 (bvchop 48 ad2))
+                    (disjoint-regionsp-spec len1 ad1 len2 ad2))
+           :hints (("Goal"  :expand (disjoint-regionsp-spec len1 ad1 len2 ad2)
+                    :in-theory (enable ;disjoint-regionsp-spec
+                                 )))))
+
+  (local (defthmd disjoint-regionsp-spec-of-bvchop-arg4-bk
+           (implies (disjoint-regionsp-spec len1 ad1 len2 ad2)
+                    (disjoint-regionsp-spec len1 ad1 len2 (bvchop 48 ad2)))
+           :hints (("Goal" :expand (disjoint-regionsp-spec len1 ad1 len2 (bvchop 48 ad2))
+                    :in-theory (enable ;disjoint-regionsp-spec
+                                 )))))
+
+  (defthm disjoint-regionsp-spec-of-bvchop-arg4
+    (equal (disjoint-regionsp-spec len1 ad1 len2 (bvchop 48 ad2))
+           (disjoint-regionsp-spec len1 ad1 len2 ad2))
+    :hints (("Goal" :use (disjoint-regionsp-spec-of-bvchop-arg4-fw
+                           disjoint-regionsp-spec-of-bvchop-arg4-bk)))))
+
 (defthm disjoint-regionsp-spec-of-one-smaller
   (implies (and (not (zp len1))
                 (disjoint-regionsp-spec len1 ad1 len2 ad2)
-                (unsigned-byte-p 48 len1)
-                (unsigned-byte-p 48 len2)
+        ;        (unsigned-byte-p 48 len1)
+         ;       (unsigned-byte-p 48 len2)
                 (unsigned-byte-p 48 ad1)
                 (unsigned-byte-p 48 ad2))
            (disjoint-regionsp-spec (+ -1 len1) (bvplus 48 1 ad1) len2 ad2))
@@ -425,72 +499,67 @@
                            (disjoint-regionsp-spec-necc-better
                             disjoint-regionsp-spec-necc-better-alt)))))
 
-(defthm disjoint-regionsp-when-zp
-  (implies (and (zp len1)
-                (natp len1) ; drop, have the function nfix
-                )
-           (disjoint-regionsp len1 ad1 len2 ad2))
-  :hints (("Goal" :in-theory (enable disjoint-regionsp zp))))
-
 (local (defun indf (n ad) (if (zp n) (list n ad) (indf (+ -1 n) (bvplus 48 1 ad)))))
 
 (defthmd disjoint-regionsp-opener
   (implies (and (posp len1)
-                (unsigned-byte-p 48 len1)
-                (unsigned-byte-p 48 len2)
+         ;       (unsigned-byte-p 48 len1)
+          ;      (unsigned-byte-p 48 len2)
                 (unsigned-byte-p 48 ad1)
-                (unsigned-byte-p 48 ad2))
+;                (unsigned-byte-p 48 ad2)
+                )
            (equal (disjoint-regionsp len1 ad1 len2 ad2)
                   (and (not (in-regionp ad1 len2 ad2))
                        (disjoint-regionsp (+ -1 len1) (+ 1 ad1) len2 ad2))))
     :hints (("Goal" :in-theory (enable disjoint-regionsp in-regionp bvlt bvplus bvminus bvuminus acl2::bvchop-of-sum-cases))))
 
-(in-theory (disable disjoint-regionsp-spec))
-
 (defthm disjoint-regionsp-correct-backward
   (implies (and (disjoint-regionsp-spec len1 ad1 len2 ad2)
-                ;(natp len1)
-                (unsigned-byte-p 48 len1)
-                (unsigned-byte-p 48 len2)
                 (unsigned-byte-p 48 ad1)
                 (unsigned-byte-p 48 ad2))
            (disjoint-regionsp len1 ad1 len2 ad2))
   :hints (("Goal" :induct (indf len1 ad1)
            :in-theory (enable disjoint-regionsp-opener
-                              disjoint-regionsp-of-+-arg2))))
+                              disjoint-regionsp-of-+-arg2
+                              zp natp))))
 
 (defthm disjoint-regionsp-correct-forward
   (implies (disjoint-regionsp len1 ad1 len2 ad2)
            (disjoint-regionsp-spec len1 ad1 len2 ad2))
   :hints (("Goal" :in-theory (enable disjoint-regionsp-spec))))
 
+;; Shows that the complicated defintion of disjoint-regionsp agrees with the higher-level spec.
 (defthm disjoint-regionsp-correct
-  (implies (and (unsigned-byte-p 48 len1)
-                (unsigned-byte-p 48 len2)
-                (unsigned-byte-p 48 ad1)
-                (unsigned-byte-p 48 ad2))
-           (equal (disjoint-regionsp-spec len1 ad1 len2 ad2)
-                  (disjoint-regionsp len1 ad1 len2 ad2)))
-  :hints (("Goal" :use (disjoint-regionsp-correct-forward
-                         disjoint-regionsp-correct-backward)
+  (equal (disjoint-regionsp-spec len1 ad1 len2 ad2)
+         (disjoint-regionsp len1 ad1 len2 ad2))
+  :hints (("Goal" :use ((:instance disjoint-regionsp-correct-forward (ad1 (bvchop 48 ad1)) (ad2 (bvchop 48 ad2)))
+                        (:instance disjoint-regionsp-correct-backward (ad1 (bvchop 48 ad1)) (ad2 (bvchop 48 ad2))))
            :in-theory (disable disjoint-regionsp-correct-forward
                                disjoint-regionsp-correct-backward))))
 
 ;;;;;;;;;;;;;;;;;;;;;;;;;;;;;;;;;;;;;;;;;;;;;;;;;;;;;;;;;;;;;;;;;;;;;;;;;;;;;;;;
 
-;; Checks whether all of the addresses in the first region are in the second region
+;; Checks whether all of the addresses in the first region (of size len1 starting at ad1) are in the second region (of size len2 starting at ad2).
 ;; We put the len args first because they will often be small constants.
+;; This can be opened to a conjunction of nice BV facts (requires opening in-regionp too).
 (defund subregionp (len1 ad1 len2 ad2)
-  (declare (xargs :guard (and (unsigned-byte-p 48 len1) ; can't be 2^48 as the len gets chopped to 48 bits
+  (declare (xargs :guard (and (natp len1) ; note that len >= 2^48 covers the whole region
                               (unsigned-byte-p 48 ad1)
-                              (unsigned-byte-p 48 len2) ; can't be 2^48 as the len gets chopped to 48 bits
+                              (natp len2) ; note that len >= 2^48 covers the whole region
                               (unsigned-byte-p 48 ad2))))
   (if (zp len1)
-      t
-    ;; both the first and last address of region1 are in region2:
-    (and (in-regionp ad1 len2 ad2)
-         (bvle 48 len1 len2) ; ensures the difference is not negative
-         (bvle 48 (bvminus 48 ad1 ad2) (bvminus 48 len2 len1)))))
+      t ; first region is empty
+    (if (zp len2)
+        nil ; second region is empty (but first is not)
+      (if (<= (expt 2 48) len2)
+          t ; second region is the whole address space
+        (if (<= (expt 2 48) len1)
+            nil ; first region is the whole address space (but second region is not)
+          ;; Normal case (non-huge, non-empty regions):
+          ;; Checks that both the first and last address of region1 are in region2:
+          (and (in-regionp ad1 len2 ad2)
+               (bvle 48 len1 len2) ; ensures the difference below is not negative
+               (bvle 48 (bvminus 48 ad1 ad2) (bvminus 48 len2 len1))))))))
 
 ;; A region is a subregion of itself
 (defthm subregionp-reflexive
@@ -518,9 +587,7 @@
 
 (defthm in-regionp-when-in-regionp-and-subregionp
   (implies (and (subregionp len1 ad1 len2 ad2)
-                (in-regionp ad len1 ad1)
-                (unsigned-byte-p 48 len1)
-                (unsigned-byte-p 48 len2))
+                (in-regionp ad len1 ad1))
            (in-regionp ad len2 ad2))
   :hints (("Goal" :in-theory (enable in-regionp disjoint-regionsp SUBREGIONP
                                      bvuminus bvplus bvlt
@@ -533,9 +600,7 @@
 ;; todo: prove from the above
 (defthm not-subregionp-when-in-regionp-and-not-in-regionp
   (implies (and (in-regionp ad len1 ad1)
-                (not (in-regionp ad len2 ad2))
-                (unsigned-byte-p 48 len1)
-                (unsigned-byte-p 48 len2))
+                (not (in-regionp ad len2 ad2)))
            (not (subregionp len1 ad1 len2 ad2)))
   :hints (("Goal" :in-theory (enable in-regionp disjoint-regionsp SUBREGIONP
                                      bvuminus bvplus bvlt
@@ -594,6 +659,7 @@
            (equal (subregionp len1 (+ x y) len2 ad2)
                   (subregionp len1 (bvplus 48 x y) len2 ad2)))
   :hints (("Goal" :in-theory (enable subregionp
+                                     in-regionp-of-+-arg1
                                      acl2::bvminus-of-+-arg2))))
 (theory-invariant (incompatible (:rewrite subregionp-of-+-arg2) (:definition bvplus)))
 
@@ -643,12 +709,12 @@
 ;;          (<= (expt 2 47) (bvchop 48 x)))
 ;;   :hints (("Goal" :in-theory (e/d (sbvlt) (logext)))))
 
-;; removes the negative part of the range
+;; ;; removes the negative part of the range
 (defthm subregionp-when-non-negative-and-negative-range
   (implies (and (<= (expt 2 47) (bvchop 48 k)) ; (sbvlt 48 k 0)
                 (unsigned-byte-p 48 k) ; drop?
                 (unsigned-byte-p 47 x) ; non-negative
-                (unsigned-byte-p 47 len1)
+;                (unsigned-byte-p 47 len1)
                 (unsigned-byte-p 47 len2) ; gen?
                 (<= (- (expt 2 48) k) len2) ;move to rhs?
                 )
@@ -673,7 +739,9 @@
 
 (defthm subregionp-of-1-arg1
   (equal (subregionp 1 x len2 y)
-         (in-regionp x len2 y))
+         (and (natp len2)
+              (or (<= (expt 2 48) len2)
+                  (in-regionp x len2 y))))
   :hints (("Goal" :in-theory (enable subregionp in-regionp bvlt bvplus bvuminus acl2::bvchop-of-sum-cases))))
 
 (defthm subregionp-subst-constant-arg4
@@ -706,21 +774,60 @@
   :hints (("Goal" :use in-regionp-when-in-regionp-and-subregionp-spec
            :in-theory (disable in-regionp-when-in-regionp-and-subregionp-spec))))
 
-(defthm subregionp-correct-forward
-  (implies (and (unsigned-byte-p 48 len1)
-                (unsigned-byte-p 48 len2))
-           (implies (subregionp len1 ad1 len2 ad2)
-                    (subregionp-spec len1 ad1 len2 ad2)))
-  :hints (("Goal"
-           :use (:instance in-regionp-when-in-regionp-and-subregionp
-                           (ad (subregionp-spec-witness len1 ad1 len2 ad2)))
-           :in-theory (e/d (subregionp-spec)
-                           (in-regionp-when-in-regionp-and-subregionp)))))
+(encapsulate ()
+  (local
+    (defthmd subregionp-spec-of-bvchop-arg2-fw
+      (implies (subregionp-spec len1 (bvchop 48 ad1) len2 ad2)
+               (subregionp-spec len1 ad1 len2 ad2))
+      :hints (("Goal" :expand (subregionp-spec len1 ad1 len2 ad2)))))
+
+  (local
+    (defthmd subregionp-spec-of-bvchop-arg2-bk
+      (implies (subregionp-spec len1 ad1 len2 ad2)
+               (subregionp-spec len1 (bvchop 48 ad1) len2 ad2))
+      :hints (("Goal" :expand (subregionp-spec len1 (bvchop 48 ad1) len2 ad2)))))
+
+  (defthm subregionp-spec-of-bvchop-arg2
+    (equal (subregionp-spec len1 (bvchop 48 ad1) len2 ad2)
+           (subregionp-spec len1 ad1 len2 ad2))
+    :hints (("Goal" :use (subregionp-spec-of-bvchop-arg2-fw
+                           subregionp-spec-of-bvchop-arg2-bk)))))
+
+(encapsulate ()
+  (local
+    (defthmd subregionp-spec-of-bvchop-arg4-fw
+      (implies (subregionp-spec len1 ad1 len2 (bvchop 48 ad2))
+               (subregionp-spec len1 ad1 len2 ad2))
+      :hints (("Goal" :expand (subregionp-spec len1 ad1 len2 ad2)))))
+
+  (local
+    (defthmd subregionp-spec-of-bvchop-arg4-bk
+      (implies (subregionp-spec len1 ad1 len2 ad2)
+               (subregionp-spec len1 ad1 len2 (bvchop 48 ad2)))
+      :hints (("Goal" :expand (subregionp-spec len1 ad1 len2 (bvchop 48 ad2))))))
+
+  (defthm subregionp-spec-of-bvchop-arg4
+    (equal (subregionp-spec len1 ad1 len2 (bvchop 48 ad2))
+           (subregionp-spec len1 ad1 len2 ad2))
+    :hints (("Goal" :use (subregionp-spec-of-bvchop-arg4-fw
+                           subregionp-spec-of-bvchop-arg4-bk)))))
+
+(local
+  (defthm subregionp-correct-forward
+    (implies (subregionp len1 ad1 len2 ad2)
+             (subregionp-spec len1 ad1 len2 ad2))
+    :hints (("Goal"
+             :use (:instance in-regionp-when-in-regionp-and-subregionp
+                             (ad (subregionp-spec-witness len1 ad1 len2 ad2)))
+             :in-theory (e/d (subregionp-spec)
+                             (in-regionp-when-in-regionp-and-subregionp))))))
 
 (local
   (defthm subregionp-spec-same-ads-forward
-    (implies (and (unsigned-byte-p 48 len1)
-                  (unsigned-byte-p 48 len2))
+    (implies (and; (unsigned-byte-p 48 len1)
+               (natp len1)
+               (unsigned-byte-p 48 len2)
+               )
              (implies (subregionp-spec len1 ad len2 ad)
                       (<= len1 len2)))
     :hints (("Goal" :use (:instance not-subregionp-spec-when-in-regionp-and-not-in-regionp
@@ -733,7 +840,8 @@
 (local
   (defthm subregionp-spec-same-ads-backward
     (implies (and (unsigned-byte-p 48 len1)
-                  (unsigned-byte-p 48 len2))
+                  (unsigned-byte-p 48 len2)
+                  )
              (implies (<= len1 len2)
                       (subregionp-spec len1 ad len2 ad)))
     :hints (("Goal" :in-theory (enable SUBREGIONP-SPEC)))))
@@ -747,17 +855,9 @@
 ;todo: make some stuff here local:
 ;todo: move some of this up:
 
-;; The bad guy is an address in r1 but not in r2, is there if such an address
-;; (defun bad-guy (r1 r2)
-;;   (if (zp (len r1))
-;;       nil
-;;     (if (member-equal (first r1) r2)
-;;         (bad-guy (rest r1) (remove1-equal (first r1) r2))
-;;       (first r1))))
-
 (defthmd subregionp-opener
-  (implies (and (unsigned-byte-p 48 len1)
-                (unsigned-byte-p 48 len2)
+  (implies (and ;(unsigned-byte-p 48 len1)
+                ;(unsigned-byte-p 48 len2)
                 (integerp ad1)
                 (not (zp len1)))
            (equal (subregionp len1 ad1 len2 ad2)
@@ -766,50 +866,58 @@
   :hints (("Goal" :in-theory (enable subregionp in-regionp bvlt bvplus bvminus bvuminus acl2::bvchop-of-sum-cases))))
 
 ;; The bad guy is an address in r1 but not in r2, is there if such an address
-(defund bad-guy (len1 ad1 len2 ad2)
-  (if (zp len1)
-      nil
-    (if (in-regionp ad1 len2 ad2)
-        ;; keep looking:
-        (bad-guy (+ -1 len1) (bvplus 48 1 ad1) len2 ad2)
-      ;; we found a bad guy:
-      ad1)))
+(local
+  (defund bad-guy (len1 ad1 len2 ad2)
+    (if (zp len1)
+        nil
+      (if (in-regionp ad1 len2 ad2)
+          ;; keep looking:
+          (bad-guy (+ -1 len1) (bvplus 48 1 ad1) len2 ad2)
+        ;; we found a bad guy:
+        ad1))))
 
-(defthm unsigned-byte-p-of-bad-guy
-  (implies (and (bad-guy len1 ad1 len2 ad2)
-                (unsigned-byte-p 48 ad1))
-           (unsigned-byte-p 48 (bad-guy len1 ad1 len2 ad2)))
-  :hints (("Goal" :in-theory (enable bad-guy))))
+(local
+  (defthm unsigned-byte-p-of-bad-guy
+    (implies (and (bad-guy len1 ad1 len2 ad2)
+                  (unsigned-byte-p 48 ad1))
+             (unsigned-byte-p 48 (bad-guy len1 ad1 len2 ad2)))
+    :hints (("Goal" :in-theory (enable bad-guy)))))
 
-(defthm in-regionp-of-bad-guy
-  (implies (and (bad-guy len1 ad1 len2 ad2)
-                ;(integerp ad1)
-                (unsigned-byte-p 48 ad1)
-                (unsigned-byte-p 48 ad2)
-                (unsigned-byte-p 48 len1))
-           (in-regionp (bad-guy len1 ad1 len2 ad2) len1 ad1))
-  :hints (("Goal" :in-theory (enable in-regionp-opener bad-guy in-regionp-of-+-arg3))))
+(local
+  (defthm in-regionp-of-bad-guy
+    (implies (and (bad-guy len1 ad1 len2 ad2)
+                  ;(integerp ad1)
+                  (unsigned-byte-p 48 ad1)
+                  (unsigned-byte-p 48 ad2)
+                  ;(unsigned-byte-p 48 len1)
+                  (natp len1)
+                  )
+             (in-regionp (bad-guy len1 ad1 len2 ad2) len1 ad1))
+    :hints (("Goal" :in-theory (enable in-regionp-opener bad-guy in-regionp-of-+-arg3)))))
 
-(defthm subregionp-when-in-regionp-of-bad-guy
-  (implies (and (in-regionp (bad-guy len1 ad1 len2 ad2) len2 ad2)
-                (unsigned-byte-p 48 len1)
-                (unsigned-byte-p 48 len2)
-                (integerp ad1))
-           (subregionp len1 ad1 len2 ad2))
-  :hints (("Goal" :in-theory (enable subregionp-opener bad-guy subregionp-of-+-arg2))))
+(local
+  (defthm subregionp-when-in-regionp-of-bad-guy
+    (implies (and (in-regionp (bad-guy len1 ad1 len2 ad2) len2 ad2)
+                  ;(unsigned-byte-p 48 len1)
+                  (natp len1)
+;                (unsigned-byte-p 48 len2)
+                  (integerp ad1))
+             (subregionp len1 ad1 len2 ad2))
+    :hints (("Goal" :in-theory (enable subregionp-opener bad-guy subregionp-of-+-arg2)))))
 
-(defthm subregionp-when-not-bad-guy
-  (implies (and (not (bad-guy len1 ad1 len2 ad2))
-                (unsigned-byte-p 48 len1)
-                (unsigned-byte-p 48 len2)
-                (integerp ad1))
-           (subregionp len1 ad1 len2 ad2))
-  :hints (("Goal" :in-theory (enable subregionp-opener bad-guy subregionp-of-+-arg2))))
+(local
+  (defthm subregionp-when-not-bad-guy
+    (implies (and (not (bad-guy len1 ad1 len2 ad2))
+        ;        (unsigned-byte-p 48 len1)
+        ;       (unsigned-byte-p 48 len2)
+                  (integerp ad1))
+             (subregionp len1 ad1 len2 ad2))
+    :hints (("Goal" :in-theory (enable subregionp-opener bad-guy subregionp-of-+-arg2)))))
 
 ;drop some hyps?
-(defthm subregionp-correct-back
-  (implies (and (unsigned-byte-p 48 len1)
-                (unsigned-byte-p 48 len2)
+(defthmd subregionp-correct-back
+  (implies (and (natp len1) ;(unsigned-byte-p 48 len1)
+               ; (unsigned-byte-p 48 len2)
                 (unsigned-byte-p 48 ad1)
                 (unsigned-byte-p 48 ad2))
            (implies (subregionp-spec len1 ad1 len2 ad2)
@@ -819,14 +927,10 @@
            :in-theory (enable subregionp-opener))))
 
 ;; Our subregionp function matches the spec
-;; todo: drop some hyps?
 (defthm subregionp-correct
-  (implies (and (unsigned-byte-p 48 len1)
-                (unsigned-byte-p 48 len2)
-                (unsigned-byte-p 48 ad1)
-                (unsigned-byte-p 48 ad2))
-           (equal (subregionp-spec len1 ad1 len2 ad2)
-                  (subregionp len1 ad1 len2 ad2))))
+  (equal (subregionp-spec len1 ad1 len2 ad2)
+         (subregionp len1 ad1 len2 ad2))
+  :hints (("Goal" :use (:instance subregionp-correct-back (ad1 (bvchop 48 ad1)) (ad2 (bvchop 48 ad2))))))
 
 ;todo: show that a larger region can't be a subregion of a smaller region
 
@@ -837,10 +941,11 @@
   (implies (and (disjoint-regionsp len1 ad1 len2 ad2)
                 (subregionp len3 ad3 len1 ad1) ; expand to bv ops?
                 (subregionp len4 ad4 len2 ad2) ; expand to bv ops?
-                (unsigned-byte-p 48 len1)
-                (unsigned-byte-p 48 len2)
-                (unsigned-byte-p 48 len3)
-                (unsigned-byte-p 48 len4))
+                ;(unsigned-byte-p 48 len1)
+                ;(unsigned-byte-p 48 len2)
+                ;(unsigned-byte-p 48 len3)
+                ;(unsigned-byte-p 48 len4)
+                )
            (disjoint-regionsp len3 ad3 len4 ad4))
   :hints (("Goal"
            :in-theory (enable in-regionp disjoint-regionsp subregionp
@@ -854,9 +959,10 @@
   (implies (and (disjoint-regionsp len2 ad2 len1 ad1)
                 (subregionp len3 ad3 len1 ad1) ; expand to bv ops?
                 (subregionp len4 ad4 len2 ad2) ; expand to bv ops?
-                (unsigned-byte-p 48 len1)
-                (unsigned-byte-p 48 len2)
-                (unsigned-byte-p 48 len3)
-                (unsigned-byte-p 48 len4))
+                ;(unsigned-byte-p 48 len1)
+                ;(unsigned-byte-p 48 len2)
+                ;(unsigned-byte-p 48 len3)
+                ;(unsigned-byte-p 48 len4)
+                )
            (disjoint-regionsp len3 ad3 len4 ad4))
   :hints (("Goal" :in-theory (enable disjoint-regionsp-symmetric))))
